Stabilizing functions

theories/Tools.v
@@ -7,11 +7,13 @@ From Stdlib Require Export ZArith.ZArith.
 From Stdlib Require Export micromega.Lia.
 From Stdlib Require Lists.List.
 Export Stdlib.Lists.List.ListNotations.
-From Corelib Require Import Program.Basics.
+From Corelib Require Export Program.Basics.
+From Stdlib Require Export Classes.EquivDec.
 
 #[global] Obligation Tactic := ().
 Unset Program Cases.
 
+Open Scope equiv_scope.
 Open Scope list_scope.
 Open Scope Z_scope.
 Open Scope nat_scope.
@@ -31,8 +33,7 @@ Notation "x ≤ y ≤ z" := (x ≤ y /\ y ≤ z)%Z : Z_scope.
 Notation "x ≤ y < z" := (x ≤ y /\ y < z)%Z : Z_scope.
 Notation "x < y ≤ z" := (x < y /\ y ≤ z)%Z : Z_scope.
 
-(* Require Import List.
-Print In. *)
+Instance dec_eq_Z : EqDec Z eq := Z.eq_dec.
 
 Inductive mem_index {A} (a : A) : list A → Type :=
   | MIO : ∀ l', mem_index a (a :: l')
@@ -42,9 +43,47 @@ Arguments MIS {A a b l'}.
 
 Check MIS (MIS (MIS MIO)).
 
-(* Declare Scope typed_index_scope.
-Delimit Scope typed_index_scope with typed_index.
-Bind Scope typed_index_scope with typed_index.
-Open Scope typed_index_scope.
+Definition stabilizing {A B} (f : A → B) :=
+  ∃ l b, ∀ a, List.In a l ∨ f a = b.
 
-Number Notation typed_index True True : typed_index_scope. *)
+Record stabilizing_fun A B := {
+  stabilizing_fun_f :> A → B;
+  stabilizing_fun_stabilizing_f : stabilizing stabilizing_fun_f;
+}.
+Arguments stabilizing_fun_f {A B}.
+Arguments stabilizing_fun_stabilizing_f {A B}.
+
+Notation "A  '→₀'  B" := (stabilizing_fun A B) (at level 99, right associativity) : type_scope.
+
+Lemma injective_stabilizing_fun_f {A B} :
+  ∀ f g : A →₀ B, stabilizing_fun_f f = stabilizing_fun_f g → f = g.
+Proof.
+  intros f g H. destruct f as [f stabilizing_f], g as [g stabilizing_g].
+  simpl in H. destruct H. f_equal. apply proof_irrelevance.
+Qed.
+
+#[program]
+Definition stabilizing_fun_const {A B} b : A →₀ B := {|
+  stabilizing_fun_f := λ _, b;
+|}.
+Next Obligation.
+  intros A B b. exists [], b. intros a. auto.
+Qed.
+
+#[program]
+Definition stabilizing_fun_update {A B} `{equiv : Equivalence A eq} `{dec_equiv : @EqDec A eq equiv} (f : A →₀ B) a b := {|
+  stabilizing_fun_f := λ a', if a' == a then b else f a';
+|}.
+Next Obligation.
+  intros A B equiv dec_equiv f a b. destruct f as [f (l & b' & H_f)]. exists (a :: l), b'. intros a'. simpl. destruct (a' == a) as [H_a' | H_a'].
+  - left. left. auto.
+  - specialize (H_f a'). destruct H_f; auto.
+Qed.
+
+Declare Scope stabilizing_fun_scope.
+Delimit Scope stabilizing_fun_scope with stabilizing_fun.
+Bind Scope stabilizing_fun_scope with stabilizing_fun.
+Open Scope stabilizing_fun_scope.
+
+Notation "'_'  '↦₀'  b" := (stabilizing_fun_const b) (at level 70) : stabilizing_fun_scope.
+Notation "a  '↦₀'  b ','  f" := (stabilizing_fun_update f a b) (at level 70, f at level 200) : stabilizing_fun_scope.
