theories/PCFm.v
@@ -2,15 +2,11 @@ From PCF Require Import Tools.
 From PCF Require Import Zm.
 From PCF Require Import Types.
 
-Unset Positivity Checking.
-
-Axiom FinFun : Type → Type → Type.
-
 Inductive termₘ μ : list type → type → Type :=
   | Oₘ : ∀ Γ, termₘ μ Γ ι
   | predₘ : ∀ Γ, termₘ μ Γ (ι ⇒ ι)
   | succₘ : ∀ Γ, termₘ μ Γ (ι ⇒ ι)
-  | matchₘ : ∀ Γ, termₘ μ Γ ι → FinFun (Zm μ) (termₘ μ Γ ι) → termₘ μ Γ ι
+  | switchₘ : ∀ Γ, termₘ μ Γ ι → (Zm μ →₀ termₘ μ Γ ι) → termₘ μ Γ ι
   | fixₘ : ∀ Γ α, termₘ μ Γ ((α ⇒ α) ⇒ α)
   | Varₘ : ∀ Γ α, mem_index α Γ → termₘ μ Γ α
   | Appₘ : ∀ Γ α β, termₘ μ Γ (α ⇒ β) → termₘ μ Γ α → termₘ μ Γ β
@@ -18,7 +14,7 @@ Inductive termₘ μ : list type → type → Type :=
 Arguments Oₘ {μ Γ}.
 Arguments predₘ {μ Γ}.
 Arguments succₘ {μ Γ}.
-Arguments matchₘ {μ Γ}.
+Arguments switchₘ {μ Γ}.
 Arguments fixₘ {μ Γ}.
 Arguments Varₘ {μ Γ}.
 Arguments Appₘ {μ Γ α β}.
@@ -29,3 +25,5 @@ Notation "'λₘ:'  α ','  s" := (Absₘ α s) (at level 35, s at level 200).
 
 Check (λₘ: ι, λₘ: ι, Varₘ ι (MIS MIO)) $ₘ (succₘ $ₘ Varₘ ι MIO) $ₘ Oₘ.
 (* Check (λₘ: ι, λₘ: ι, Varₘ ι (MIS MIO)) $ₘ (λₘ: ι, Varₘ ι MIO). *)
+
+Check λₘ: ι, switchₘ (Varₘ ι MIO) (Zm_of_Z 0 ↦₀ succₘ $ₘ (succₘ $ₘ Oₘ), Zm_of_Z 1 ↦₀ Oₘ, _ ↦₀ succₘ $ₘ Oₘ).
